src/HOL/IMP/Vars.thy
@@ -2,7 +2,7 @@
 
 header "Definite Initialization Analysis"
 
-theory Vars imports BExp
+theory Vars imports Com
 begin
 
 subsection "The Variables in an Expression"
@@ -66,5 +66,30 @@ proof(induction b)
   hence "aval a1 s\<^isub>1 = aval a1 s\<^isub>2" and "aval a2 s\<^isub>1 = aval a2 s\<^isub>2" by simp_all
   thus ?case by simp
 qed simp_all
+
+
+instantiation com :: vars
+begin
+
+fun vars_com :: "com \<Rightarrow> vname set" where
+"vars com.SKIP = {}" |
+"vars (x::=e) = {x} \<union> vars e" |
+"vars (c1;c2) = vars c1 \<union> vars c2" |
+"vars (IF b THEN c1 ELSE c2) = vars b \<union> vars c1 \<union> vars c2" |
+"vars (WHILE b DO c) = vars b \<union> vars c"
+
+instance ..
+
+end
+
+
+lemma finite_avars[simp]: "finite(vars(a::aexp))"
+by(induction a) simp_all
+
+lemma finite_bvars[simp]: "finite(vars(b::bexp))"
+by(induction b) (simp_all add: finite_avars)
+
+lemma finite_cvars[simp]: "finite(vars(c::com))"
+by(induction c) (simp_all add: finite_avars finite_bvars)
 
 end
